README.md
@@ -1,0 +1,4 @@
+categorical-unification
+==
+
+An exploration of unification implemented on the categorical representation of terms.
